specs/L2AssetRouter/L2AssetRouter/Common/block_8329248737440719504_user.lean
@@ -11,12 +11,13 @@ section
 
 open Clear EVMState Ast Expr Stmt FunctionDefinition State Interpreter ExecLemmas OutOfFuelLemmas Abstraction YulNotation PrimOps ReasoningPrinciple Utilities generated.L2AssetRouter L2AssetRouter
 
-def A_block_8329248737440719504 (s₀ s₉ : State) : Prop := sorry
+def A_block_8329248737440719504 (s₀ s₉ : State) : Prop := block_8329248737440719504_concrete_of_code.1 s₀ s₉
 
 lemma block_8329248737440719504_abs_of_concrete {s₀ s₉ : State} :
   Spec block_8329248737440719504_concrete_of_code s₀ s₉ →
   Spec A_block_8329248737440719504 s₀ s₉ := by
-  sorry
+  intro h
+  simpa [A_block_8329248737440719504] using h
 
 end
 
