specs/L2AssetRouter/L2AssetRouter/Common/if_238091860639932951_user.lean
@@ -13,12 +13,13 @@ section
 
 open Clear EVMState Ast Expr Stmt FunctionDefinition State Interpreter ExecLemmas OutOfFuelLemmas Abstraction YulNotation PrimOps ReasoningPrinciple Utilities L2AssetRouter.Common generated.L2AssetRouter L2AssetRouter
 
-def A_if_238091860639932951 (s₀ s₉ : State) : Prop := sorry
+def A_if_238091860639932951 (s₀ s₉ : State) : Prop := if_238091860639932951_concrete_of_code.1 s₀ s₉
 
 lemma if_238091860639932951_abs_of_concrete {s₀ s₉ : State} :
   Spec if_238091860639932951_concrete_of_code s₀ s₉ →
   Spec A_if_238091860639932951 s₀ s₉ := by
-  sorry
+  intro h
+  simpa [A_if_238091860639932951] using h
 
 end
 
